cava/Cava/Lib/Retiming.v
@@ -20,6 +20,7 @@ Require Import Cava.Core.Core.
 Require Import Cava.Semantics.Combinational.
 Require Import Cava.Semantics.Equivalence.
 Require Import Cava.Semantics.Simulation.
+Require Import Cava.Semantics.Loopless.
 Require Import Cava.Semantics.WeakEquivalence.
 Require Import Cava.Lib.CircuitTransforms.
 Require Import Cava.Lib.Combinators.
@@ -30,119 +31,25 @@ Section WithCava.
   Context `{semantics : Cava}.
 
   (* make a circuit with one delay for each signal, given reset values *)
-  Fixpoint delays {t : type} : value (signal:=combType) t -> Circuit t t :=
+  Fixpoint delays {t : type} : Circuit t t :=
     match t with
-    | tzero => fun _ => Id
-    | tone t => DelayInit
-    | tpair t1 t2 => fun v => Par (delays (fst v)) (delays (snd v))
-    end.
-
-  (* get the value stored in the 1-delay circuit *)
-  Fixpoint delays_get {t : type}
-    : forall {v : value t}, value (circuit_state (delays v)) -> value t :=
-    match t with
-    | tzero => fun _ _ => tt
-    | tone _ => fun _ => snd
-    | tpair _ _ => fun _ st => (delays_get (fst st), delays_get (snd st))
+    | tzero => Id
+    | tone t => Delay
+    | tpair t1 t2 => Par delays delays
     end.
 
   (* make a circuit with repeated delays for each signal *)
-  Fixpoint ndelays {t : type} (v : list (value (signal:=combType) t)) : Circuit t t :=
-    match v with
-    | [] => Id
-    | v0 :: v => ndelays v >==> delays v0
+  Fixpoint ndelays {t : type} (n : nat) : Circuit t t :=
+    match n with
+    | 0 => Id
+    | S m => ndelays m >==> delays
     end.
-
-  (* get all the values stored in the n-delay circuit *)
-  Fixpoint ndelays_get {t v} : value (circuit_state (@ndelays t v)) -> list (value t) :=
-    match v with
-    | [] => fun _ => []
-    | _ :: _ => fun st => delays_get (snd st) :: ndelays_get (fst st)
-    end.
-
 End WithCava.
 
-Inductive is_delays : forall {t}, Circuit t t -> Prop :=
-| is_delays_delay : forall t resetval, is_delays (DelayInit (t:=t) resetval)
-| is_delays_par :
-    forall t1 t2 c1 c2,
-      is_delays c1 -> is_delays c2 ->
-      @is_delays (t1 * t2) (Par c1 c2)
-.
-
-Inductive is_ndelays : forall {t}, nat -> Circuit t t -> Prop :=
-| is_ndelays_id : forall t, is_ndelays (t:=t) 0 Id
-| is_ndelays_compose :
-    forall t n c1 c2,
-      is_ndelays (t:=t) n c1 -> is_delays c2 ->
-      is_ndelays (S n) (c1 >==> c2)
-.
-
-Definition retimed {i o} (n : nat) (c1 c2 : Circuit i o) : Prop :=
-  exists delay_circuit,
-    is_ndelays n delay_circuit
-    /\ cequiv c1 (delay_circuit >==> c2).
-
-Fixpoint loops_state {i o} (c : Circuit i o) : type :=
-  match c with
-  | Comb _ => tzero
-  | First f => loops_state f
-  | Second f => loops_state f
-  | Compose f g => loops_state f * loops_state g
-  | @DelayInitCE _ _ t _ => tzero
-  | @LoopInitCE _ _ _ _ t _ body => loops_state body * t
-  end.
-
-Fixpoint loops_reset_state {i o} (c : Circuit i o)
-  : value (signal:=combType) (loops_state c) :=
-  match c with
-  | Comb _ => tt
-  | First f => loops_reset_state f
-  | Second f => loops_reset_state f
-  | Compose f g => (loops_reset_state f, loops_reset_state g)
-  | DelayInitCE _=> tt
-  | LoopInitCE resetval body => (loops_reset_state body, resetval)
-  end.
-
-Require Import ExtLib.Structures.Monad.
-Import MonadNotation.
-
-(* Pull the loops out of the circuit completely *)
-Fixpoint loopless {i o} (c : Circuit i o)
-  : Circuit (i * loops_state c) (o * loops_state c) :=
-  match c as c in Circuit i o
-        return Circuit (i * loops_state c) (o * loops_state c) with
-  | Comb f => First (Comb f)
-  | First f =>
-    Comb (i:=(_*_*_)) (fun '(x1,x2,st) => ret (x1,st,x2)) (* rearrange *)
-         >==> First (loopless f) (* recursive call *)
-         >==> Comb (i:=(_*_*_)) (fun '(y1,st,y2) => ret (y1,y2,st)) (* rearrange *)
-  | Second f =>
-    Comb (i:=(_*_*_)) (fun '(x1,x2,st) => ret (x1,(x2,st))) (* rearrange *)
-         >==> Second (loopless f) (* recursive call *)
-         >==> Comb (i:=(_*(_*_))) (fun '(y1,(y2,st)) => ret (y1,y2,st)) (* rearrange *)
-  | Compose f g =>
-    Comb (i:=(_*(_*_))) (fun '(x,(st1,st2)) => ret (x,st1,st2)) (* rearrange *)
-         >==> First (loopless f) (* recursive call *)
-         >==> Comb (i:=(_*_*_)) (fun '(y,st1,st2) => ret (y,st2,st1)) (* rearrange *)
-         >==> First (loopless g) (* recursive call *)
-         >==> Comb (i:=(_*_*_))  (fun '(z,st2,st1) => ret (z,(st1,st2))) (* rearrange *)
-  | DelayInitCE resetval => First (DelayInitCE resetval)
-  | @LoopInitCE _ _ _ _ s resetval body =>
-    (Comb (i:=(_*_*(_*_)))
-          (fun '(x,en,(body_st, loop_st)) =>
-             ret (en,loop_st,(x,loop_st,body_st)))) (* rearrange *)
-         >==> Second (loopless body) (* recursive call *)
-         >==> (Comb (i:=(Bit * _ * (_ * _ * _))) (o:=(_*(_* _)))
-                    (fun '(en, loop_st, (y, loop_st', body_st')) =>
-                       loop_st' <- mux2 en (loop_st,loop_st') ;;
-                       ret (y,(body_st',loop_st'))))
-  end.
-
+(* n is delays on state; m is delays on input *)
 Definition phase_retimed {i o} (n m : nat) (c1 c2 : Circuit i o) : Prop :=
-  exists state_resets input_resets,
-    length state_resets = n
-    /\ length input_resets = m
-    /\ cequiv c1 (LoopInit (loops_reset_state c2)
-                          (Par (ndelays input_resets) (ndelays state_resets)
-                           >==> loopless c2)).
+  exists (proj21 : value (loops_state c2) -> value (loops_state c1))
+    (proj12 : value (loops_state c1) -> value (loops_state c2)),
+    (forall x, proj12 (proj21 x) = x)
+    /\ wequiv (Second (Comb proj21) >==> loopless c1 >==> Second (Comb proj12))
+             (Par (ndelays m) (ndelays n)  >==> loopless c2).
