cava/Cava/Semantics/WeakEquivalence.v
@@ -22,283 +22,96 @@ Require Import Cava.Core.Core.
 Require Import Cava.Semantics.Combinational.
 Require Import Cava.Semantics.Equivalence.
 Require Import Cava.Semantics.Simulation.
+Require Import Cava.Semantics.Loopless.
+Require Import Cava.Semantics.LooplessProperties.
 Require Import Cava.Util.List.
 Require Import Cava.Util.Tactics.
 Import Circuit.Notations.
 
-(* get the state of a circuit after running it on the specified input from the
-   specified start state *)
-Definition repeat_step {i o} (c : Circuit i o) input st : value (circuit_state c) :=
-  fold_left (fun st i => fst (step c st i)) input st.
-
-(* Circuit equivalence relation that allows the first n timesteps to differ *)
+(* Circuit equivalence relation that stipulates an equal output after n timesteps *)
 Definition cequivn {i o} (n : nat) (c1 c2 : Circuit i o) : Prop :=
-  (* there exists some relation between the circuit states... *)
-  exists (R : value (circuit_state c1) -> value (circuit_state c2) -> Prop),
-    (* ...and the relation holds after n timesteps of equal input for all inputs
-       and all initial states *)
-    (forall input st1 st2,
-        length input = n ->
-        R (repeat_step c1 input st1) (repeat_step c2 input st2))
-    (* ...and if the relation holds, stepping each circuit on the same input
-         results in the same output as well as new states on which the relation
-         continues to hold *)
-    /\ (forall s1 s2 input,
-          R s1 s2 ->
-          snd (step c1 s1 input) = snd (step c2 s2 input)
-          /\ R (fst (step c1 s1 input)) (fst (step c2 s2 input))).
+  (* there exists some relation between the circuit states and a counter... *)
+  exists (R : nat -> value (circuit_state c1) -> value (circuit_state c2) -> Prop),
+    (* ...and after an equal input, R holds with a full counter (if n=0, then
+       the output is also equal) *)
+    (forall s1 s2 v, R n (fst (step c1 s1 v)) (fst (step c2 s2 v)))
+    (* ...and if n happens to be 0, then the outputs are equal on equal input *)
+    /\ (n = 0 -> forall s1 s2 v, snd (step c1 s1 v) = snd (step c2 s2 v))
+    (* ...and if the relation holds for a one counter, outputs are equal
+       regardless of input *)
+    /\ (forall s1 s2 v1 v2, R 1 s1 s2 -> snd (step c1 s1 v1) = snd (step c2 s2 v2))
+    (* ...and if the relation holds for a nonzero counter, it holds on new
+       states with a decremented counter regardless of input *)
+    /\ (forall m s1 s2 v1 v2,
+          0 < m ->
+          R (S m) s1 s2 ->
+          R m (fst (step c1 s1 v1)) (fst (step c2 s2 v2))).
 
-(* cequiv is transitive *)
-Global Instance Transitive_cequivn {i o} n : Transitive (@cequivn i o n) | 10.
-Proof.
-  intros x y z [Rxy [? Hxy]] [Ryz [? Hyz]]. logical_simplify.
-  exists (fun (st1 : value (circuit_state x)) (st2 : value (circuit_state z)) =>
-       exists st3 : value (circuit_state y), Rxy st1 st3 /\ Ryz st3 st2).
-  ssplit.
-  { intro input; intros.
-    exists (fold_left (fun st i => fst (step y st i)) input (reset_state y)).
-    eauto. }
-  { intros; logical_simplify.
-    specialize (Hxy _ _ ltac:(eassumption) ltac:(eassumption)).
-    specialize (Hyz _ _ ltac:(eassumption) ltac:(eassumption)).
-    logical_simplify. ssplit; [ congruence | ]. eauto. }
-Qed.
-
-(* cequivn is symmetric *)
-Global Instance Symmetric_cequivn {i o} n : Symmetric (@cequivn i o n) | 10.
-Proof.
-  intros x y [R [? HR]]. logical_simplify.
-  exists (fun st1 st2 => R st2 st1). ssplit; [ solve [eauto] | ].
-  intros. specialize (HR _ _ ltac:(eassumption) ltac:(eassumption)).
-  logical_simplify. eauto.
-Qed.
-
-(* Note: cequivn is NOT reflexive in general! *)
-
-Lemma skipn_fold_left_accumulate {A B C} (f : B -> A -> B * C) n ls b :
-  skipn n (fold_left_accumulate f ls b)
-  = fold_left_accumulate
-      f (skipn n ls) (fold_left (fun b a => fst (f b a)) (firstn n ls) b).
-Admitted.
-
-(* equivalent circuits produce the same output on the same input after n
-   timesteps *)
-Lemma simulate_cequivn {i o} n (c1 c2 : Circuit i o) :
-  cequivn n c1 c2 ->
-  forall input, skipn n (simulate c1 input) = skipn n (simulate c2 input).
-Proof.
-  intros [R [Hstart Hpreserved]]; intros. logical_simplify. cbv [simulate].
-  destr (length input <=? n); [ rewrite !skipn_all2 by length_hammer; reflexivity | ].
-  rewrite !skipn_fold_left_accumulate.
-  eapply fold_left_accumulate_double_invariant_In
-    with (I:=fun st1 st2 acc1 acc2 =>
-               R st1 st2 /\ acc1 = acc2).
-  { ssplit; eauto. apply Hstart. length_hammer. }
-  { intros; logical_simplify; subst.
-    lazymatch goal with
-    | H : forall _ _ _, R _ _ -> _ /\ _, HR : R _ _ |- context [step _ _ ?i] =>
-    let H1 := fresh in
-    let H2 := fresh in
-    specialize (H _ _ i HR); destruct H as [H1 H2];
-      rewrite ?H1, ?H2
-    end.
-    ssplit; eauto. }
-  { intros; logical_simplify; subst. reflexivity. }
-Qed.
-
-Lemma cequivn_cequiv {i o} (c1 c2 : Circuit i o) :
-  cequivn 0 c1 c2 -> cequiv c1 c2.
-Proof.
-  intros [R [Hstart Hstep]].
-  specialize (Hstart nil (reset_state c1) (reset_state c2) eq_refl).
-  cbn [fold_left] in Hstart. exists R; eauto.
-Qed.
-
-Lemma state_relation_fold_left_accumulate_step
-      i o (c1 c2 : Circuit i o) (R : _ -> _ -> Prop) :
-  (forall s1 s2 input,
-      R s1 s2 ->
-      snd (step c1 s1 input) = snd (step c2 s2 input)
-      /\ R (fst (step c1 s1 input)) (fst (step c2 s2 input))) ->
-  forall input s1 s2,
-    R s1 s2 ->
-    fold_left_accumulate (step c1) input s1
-    = fold_left_accumulate (step c2) input s2.
-Proof.
-  intro HR. intros.
-  apply fold_left_accumulate_double_invariant_In
-    with (I:=fun s1 s2 acc1 acc2 =>
-               R s1 s2 /\ acc1 = acc2).
-  { eauto. }
-  { intros s1' s2'; intros.
-    logical_simplify; subst.
-    specialize (HR s1' s2' ltac:(eassumption) ltac:(eassumption)).
-    logical_simplify; subst. ssplit; [ assumption | congruence ]. }
-  { intros; logical_simplify; subst; reflexivity. }
-Qed.
-
-Lemma state_relation_repeat_step
-      i o (c1 c2 : Circuit i o) (R : _ -> _ -> Prop) :
-  (forall s1 s2 input,
-      R s1 s2 ->
-      snd (step c1 s1 input) = snd (step c2 s2 input)
-      /\ R (fst (step c1 s1 input)) (fst (step c2 s2 input))) ->
-  forall input s1 s2,
-    R s1 s2 -> R (repeat_step c1 input s1) (repeat_step c2 input s2).
-Proof.
-  intro HR. intros. cbv [repeat_step].
-  eapply fold_left_double_invariant with (I:=R).
-  { eauto. }
-  { intros s1' s2'; intros.
-    logical_simplify; subst.
-    specialize (HR s1' s2' ltac:(eassumption) ltac:(eassumption)).
-    logical_simplify; subst; auto. }
-  { intros; logical_simplify; auto. }
-Qed.
-
-(*
-Global Instance Proper_cequivn i o n :
-  Proper (cequiv ==> cequiv ==> (fun A B => forall _ : A, B)) (@cequivn i o n).
-Proof.
-  intros a b [Rab [? Hab]] c d [Rcd [? Hcd]].
-  split.
-  { intros [Rac [? Hac]].
-    exists (fun sb sd =>
-         exists sa sc, Rab sa sb /\ Rcd sc sd /\ Rac sa sc).
-    ssplit.
-    { intros; cbn. do 2 eexists; ssplit; eauto.
-      {
-        apply state_relation_repeat_step; eauto.
-Qed.
-*)
-
-Lemma repeat_step_nil {i o} (c : Circuit i o) st : repeat_step c nil st = st.
-Proof. reflexivity. Qed.
-Hint Rewrite @repeat_step_nil using solve [eauto] : push_repeat_step.
-
-Lemma repeat_step_cons {i o} (c : Circuit i o) i0 input st :
-  repeat_step c (i0 :: input) st = repeat_step c input (fst (step c st i0)).
-Proof. reflexivity. Qed.
-Hint Rewrite @repeat_step_cons using solve [eauto] : push_repeat_step.
-
-Lemma repeat_step_app {i o} (c : Circuit i o) input1 input2 st :
-  repeat_step c (input1 ++ input2) st
-  = repeat_step c input2 (repeat_step c input1 st).
-Proof. apply fold_left_app. Qed.
-Hint Rewrite @repeat_step_app using solve [eauto] : push_repeat_step.
-
-Lemma repeat_step_compose {i t o} c1 c2 input st :
-  repeat_step (@Compose _ _ i t o c1 c2) input st
-  = (repeat_step c1 input (fst st),
-     repeat_step c2 (fold_left_accumulate (step c1) input (fst st)) (snd st)).
-Proof.
-  cbv [repeat_step]. revert st.
-  induction input; [ destruct st; reflexivity | ].
-  intros; cbn [circuit_state] in *. destruct_products; cbn [fst snd].
-  autorewrite with push_list_fold push_fold_acc.
-  rewrite IHinput. cbn [step].
-  repeat (destruct_pair_let; cbn [fst snd]).
-  reflexivity.
-Qed.
-Hint Rewrite @repeat_step_compose using solve [eauto] : push_repeat_step.
-
-Lemma repeat_step_First {i t o} (c : Circuit i o) input st :
-  repeat_step (First (t:=t) c) input st = repeat_step c (map fst input) st.
-Proof.
-  cbv [repeat_step]. revert st.
-  induction input; [ reflexivity | ].
-  intros; cbn [circuit_state] in *. destruct_products; cbn [fst snd].
-  autorewrite with push_list_fold push_fold_acc.
-  rewrite IHinput. cbn [step].
-  repeat (destruct_pair_let; cbn [fst snd]).
-  reflexivity.
-Qed.
-Hint Rewrite @repeat_step_First using solve [eauto] : push_repeat_step.
-
-Lemma repeat_step_Second {i t o} (c : Circuit i o) input st :
-  repeat_step (Second (t:=t) c) input st = repeat_step c (map snd input) st.
-Proof.
-  cbv [repeat_step]. revert st.
-  induction input; [ reflexivity | ].
-  intros; cbn [circuit_state] in *. destruct_products; cbn [fst snd].
-  autorewrite with push_list_fold push_fold_acc.
-  rewrite IHinput. cbn [step].
-  repeat (destruct_pair_let; cbn [fst snd]).
-  reflexivity.
-Qed.
-Hint Rewrite @repeat_step_Second using solve [eauto] : push_repeat_step.
 
 Lemma cequivn_compose {i t o} n m (a b : Circuit i t) (c d : Circuit t o) :
-  cequivn n a b -> cequivn m c d ->
-  cequivn (n + m) (a >==> c) (b >==> d).
-Proof.
-  intros [Rab [? Hab]] [Rcd [? Hcd]].
-  exists (fun st1 st2 => Rab (fst st1) (fst st2) /\ Rcd (snd st1) (snd st2)).
-  ssplit.
-  { intro input; intros. rewrite <-(firstn_skipn n input).
-    rewrite !repeat_step_app, !repeat_step_compose.
-    cbn [fst snd]. assert (length (firstn n input) = n) by length_hammer.
-    assert (length (skipn n input) = m) by length_hammer.
-    ssplit; [ apply state_relation_repeat_step; solve [eauto] | ].
-    erewrite state_relation_fold_left_accumulate_step by eauto.
-    match goal with H : _ |- _ => apply H; length_hammer end. }
-  { cbn [circuit_state step]. intros; logical_simplify.
-    pose proof (fun i => proj1 (Hab _ _ i ltac:(eassumption))) as Hab1.
-    pose proof (fun i => proj2 (Hab _ _ i ltac:(eassumption))) as Hab2.
-    pose proof (fun i => proj1 (Hcd _ _ i ltac:(eassumption))) as Hcd1.
-    pose proof (fun i => proj2 (Hcd _ _ i ltac:(eassumption))) as Hcd2.
-    clear Hab Hcd. logical_simplify.
-    repeat (destruct_pair_let; cbn [fst snd]).
-    rewrite ?Hab1, ?Hcd1. ssplit; eauto; [ apply Hab2 | apply Hcd2 ]. }
-Qed.
+  cequivn n a b -> cequivn m c d -> cequivn (n + m) (a >==> c) (b >==> d).
+Admitted.
 
+(* count the number of delays on the critical path of a circuit *)
+Fixpoint cpath {i o} (c : Circuit i o) : nat :=
+  match c with
+  | Comb _ => 0
+  | First f => cpath f
+  | Second f => cpath f
+  | Compose f g => cpath f + cpath g
+  | DelayInit _=> 1
+  | LoopInitCE _ body => cpath body
+  end.
 
-Lemma state_relation_repeat_step_longer
-      i o n (c1 c2 : Circuit i o) (R : _ -> _ -> Prop) :
-  (forall input s1 s2,
-      length input = n ->
-      R (repeat_step c1 input s1) (repeat_step c2 input s2)) ->
-  (forall s1 s2 input,
-      R s1 s2 ->
-      snd (step c1 s1 input) = snd (step c2 s2 input)
-      /\ R (fst (step c1 s1 input)) (fst (step c2 s2 input))) ->
-  forall input s1 s2,
-    n <= length input ->
-    R (repeat_step c1 input s1) (repeat_step c2 input s2).
+Definition cequivn_reflexive {i o} (c : Circuit i o) :
+  is_loop_free c = true -> cequivn (cpath c) c c.
 Proof.
-  intros Hstart HR. intros.
-  rewrite <-(firstn_skipn n input).
-  rewrite !repeat_step_app.
-  eapply state_relation_repeat_step; [ solve [eauto] | ].
-  eapply Hstart. length_hammer.
-Qed.
+  induction c; cbn [cpath is_loop_free].
+  { exists (fun i s1 s2 => i = 0 /\ s1 = s2).
+    ssplit; cbn [value step circuit_state]; intros; subst.
+    all:logical_simplify.
+    all:ssplit; try reflexivity.
+    all:discriminate. }
+  { rewrite Bool.andb_true_iff; intros; logical_simplify.
+    apply cequivn_compose; auto. }
+  { admit. (* applies across First *) }
+  { admit. (* applies across Second *) }
+  { discriminate. }
+  { intros. exists (fun i s1 s2 => i <= 1 /\ s1 = s2).
+    cbn [value step circuit_state].
+    ssplit; intros; logical_simplify; subst; ssplit;
+      try reflexivity; try lia. }
+Admitted.
 
-(* cequivn n c1 c2 -> cequivn n (First c1) (First c2) *)
-Global Instance Proper_First {i o t} n :
-  Proper (cequivn n ==> cequivn n) (@First _ _ i o t).
-Proof.
-  intros x y [Rxy [? Hxy]].
-  exists Rxy; ssplit.
-  { intros. rewrite !repeat_step_First.
-    match goal with H : _ |- _ => apply H; length_hammer end. }
-  { cbn [circuit_state step]. intros; logical_simplify.
-    pose proof (fun i => proj1 (Hxy _ _ i ltac:(eassumption))) as Hxy1.
-    pose proof (fun i => proj2 (Hxy _ _ i ltac:(eassumption))) as Hxy2.
-    clear Hxy. logical_simplify. repeat (destruct_pair_let; cbn [fst snd]).
-    rewrite Hxy1. ssplit; eauto. }
-Qed.
+(* Circuit equivalence relation that declares the circuits have equal critical
+   paths and, if both are loop-free, then they produce equivalent outputs for
+   equivalent inputs (delayed by the critical path number) *)
+Definition wequiv {i o} (c1 c2 : Circuit i o) : Prop :=
+  cpath c1 = cpath c2
+  /\ (is_loop_free c1 = true ->
+     is_loop_free c2 = true ->
+     cequivn (cpath c1) c1 c2).
 
-(* cequivn n c1 c2 -> cequivn n (Second c1) (Second c2) *)
-Global Instance Proper_Second {i o t} n :
-  Proper (cequivn n ==> cequivn n) (@Second _ _ i o t).
+Global Instance Equivalence_wequiv: forall {i o : type}, Equivalence (@wequiv i o) | 10.
+Admitted.
+
+Global Instance Proper_Second {i o t : type} :
+  Proper (@wequiv i o ==> @wequiv (t * i) (t * o)) Second.
+Admitted.
+
+Global Instance Proper_First {i o t : type} :
+  Proper (@wequiv i o ==> @wequiv (i * t) (o * t)) First.
+Admitted.
+
+Global Instance Proper_Compose {i o t : type} :
+  Proper (@wequiv i t ==> @wequiv t o ==> wequiv) Compose.
+Admitted.
+
+Lemma wequiv_delays {t} (r1 r2 : value t) : wequiv (DelayInit r1) (DelayInit r2).
 Proof.
-  intros x y [Rxy [? Hxy]].
-  exists Rxy; ssplit.
-  { intros. rewrite !repeat_step_Second.
-    match goal with H : _ |- _ => apply H; length_hammer end. }
-  { cbn [circuit_state step]. intros; logical_simplify.
-    pose proof (fun i => proj1 (Hxy _ _ i ltac:(eassumption))) as Hxy1.
-    pose proof (fun i => proj2 (Hxy _ _ i ltac:(eassumption))) as Hxy2.
-    clear Hxy. logical_simplify. repeat (destruct_pair_let; cbn [fst snd]).
-    rewrite Hxy1. ssplit; eauto. }
+  cbv [wequiv]. cbn [cpath is_loop_free]. ssplit; [ reflexivity | intros ].
+  intros. exists (fun i s1 s2 => i <= 1 /\ s1 = s2).
+  cbn [value step circuit_state].
+  ssplit; intros; logical_simplify; subst; ssplit;
+    try reflexivity; try lia.
 Qed.
