cava/Cava/Semantics/Simulation.v
@@ -111,75 +111,6 @@ Proof.
 Qed.
 Hint Rewrite @simulate_second using solve [eauto] : push_simulate.
 
-Lemma simulate_DelayInitCE {t} (init : value t) input :
-  simulate (DelayInitCE init) input
-  = firstn (length input)
-           (init :: (fold_left_accumulate
-                      (fun st i_en =>
-                         if (snd i_en : bool)
-                         then (fst i_en, fst i_en)
-                         else (st, st))
-                      input init)).
-Proof.
-  simsimpl. generalize init.
-  induction input; intros; [ reflexivity | ].
-  autorewrite with push_length push_firstn push_fold_acc.
-  cbn [value] in *. destruct_products; cbn [fst snd]. erewrite IHinput.
-  simsimpl. destruct_one_match; reflexivity.
-Qed.
-Hint Rewrite @simulate_DelayInitCE using solve [eauto] : push_simulate.
-
-Lemma simulate_DelayCE {t} (input : list (value t * bool)) :
-  simulate DelayCE input = firstn (length input)
-                                  (defaultValue
-                                     :: (fold_left_accumulate
-                                          (fun st i_en =>
-                                             if (snd i_en : bool)
-                                             then (fst i_en, fst i_en)
-                                             else (st, st))
-                                          input defaultValue)).
-Proof. apply simulate_DelayInitCE. Qed.
-Hint Rewrite @simulate_DelayCE using solve [eauto] : push_simulate.
-
-Lemma simulate_DelayInit {t} init (input : list (value t)) :
-  simulate (DelayInit init) input = firstn (length input) (init :: input).
-Proof.
-  cbv [DelayInit]. simpl_ident. autorewrite with push_simulate push_length.
-  erewrite fold_left_accumulate_to_seq with (default:=(defaultValue,false)).
-  eapply fold_left_accumulate_invariant_seq
-    with (I:=fun i (st : value t) acc =>
-               acc = firstn i input
-               /\ st = nth i (init :: input) defaultValue).
-  {  ssplit; reflexivity. }
-  { cbv zeta; intro i; intros. subst.
-    destruct_products; cbn [fst snd] in *.
-    logical_simplify; subst. cbn [fst snd].
-    autorewrite with push_length in *.
-    autorewrite with push_firstn push_nth pull_snoc natsimpl.
-    erewrite !map_nth_inbounds with (d2:=defaultValue) by length_hammer.
-    cbn [value] in *.  erewrite firstn_succ_snoc by lia. cbn [fst snd].
-    ssplit; reflexivity. }
-  { intros. logical_simplify; subst. cbn [fst snd].
-    autorewrite with push_length push_firstn.
-    reflexivity. }
-Qed.
-Hint Rewrite @simulate_DelayInit using solve [eauto] : push_simulate.
-
-Lemma simulate_Delay {t} (input : list (value t)) :
-  simulate Delay input = firstn (length input) (defaultValue :: input).
-Proof. apply simulate_DelayInit. Qed.
-Hint Rewrite @simulate_Delay using solve [eauto] : push_simulate.
-
-Lemma simulate_length {i o} (c : Circuit i o) input :
-  length (simulate c input) = length input.
-Proof.
-  simsimpl. generalize (reset_state c).
-  induction input; intros; [ reflexivity | ].
-  simsimpl. autorewrite with push_length.
-  reflexivity.
-Qed.
-Hint Rewrite @simulate_length using solve [eauto] : push_length.
-
 Lemma simulate_LoopInitCE {i o s}
       resetval (body : Circuit (i * s) (o * s))
       (input : list (value i * bool)) :
@@ -239,3 +170,54 @@ Lemma simulate_Loop {i o s}
     input (reset_state body, defaultValue).
 Proof. apply simulate_LoopInit. Qed.
 Hint Rewrite @simulate_Loop using solve [eauto] : push_simulate.
+
+Lemma simulate_DelayInit {t} init (input : list (value t)) :
+  simulate (DelayInit init) input = firstn (length input) (init :: input).
+Proof.
+  simsimpl. generalize init.
+  induction input; intros; [ reflexivity | ].
+  autorewrite with push_length push_firstn push_fold_acc.
+  cbn [value] in *. destruct_products; cbn [fst snd]. erewrite IHinput.
+  simsimpl. reflexivity.
+Qed.
+Hint Rewrite @simulate_DelayInit using solve [eauto] : push_simulate.
+
+Lemma simulate_DelayInitCE {t} (init : value t) input :
+  simulate (DelayInitCE init) input
+  = firstn (length input)
+           (init :: (fold_left_accumulate
+                      (fun st i_en =>
+                         if (snd i_en : bool)
+                         then (fst i_en, fst i_en)
+                         else (st, st))
+                      input init)).
+Admitted.
+Hint Rewrite @simulate_DelayInitCE using solve [eauto] : push_simulate.
+
+Lemma simulate_DelayCE {t} (input : list (value t * bool)) :
+  simulate DelayCE input = firstn (length input)
+                                  (defaultValue
+                                     :: (fold_left_accumulate
+                                          (fun st i_en =>
+                                             if (snd i_en : bool)
+                                             then (fst i_en, fst i_en)
+                                             else (st, st))
+                                          input defaultValue)).
+Proof. apply simulate_DelayInitCE. Qed.
+Hint Rewrite @simulate_DelayCE using solve [eauto] : push_simulate.
+
+
+Lemma simulate_Delay {t} (input : list (value t)) :
+  simulate Delay input = firstn (length input) (defaultValue :: input).
+Proof. apply simulate_DelayInit. Qed.
+Hint Rewrite @simulate_Delay using solve [eauto] : push_simulate.
+
+Lemma simulate_length {i o} (c : Circuit i o) input :
+  length (simulate c input) = length input.
+Proof.
+  simsimpl. generalize (reset_state c).
+  induction input; intros; [ reflexivity | ].
+  simsimpl. autorewrite with push_length.
+  reflexivity.
+Qed.
+Hint Rewrite @simulate_length using solve [eauto] : push_length.
